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Using FORM in the context of Compton scattering

A. Context

Figure (1) gives the Feynman diagrams corresponding to the two lowest-order processes contribut-

ing to Compton scattering. As per Griffiths’ (2008, Example 7.4) the probability amplitude M1

associated with the first of those Feynman diagrams is:

M1

i
=

∫
d4q

(2π)4
ǫµ(2)
︸︷︷︸

γ in







ū4
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where ū4 is the (adjoint) spinor associated with the outgoing electron, u1 is the spinor representing

the incoming electron, ǫµ(2) are the components of the polarization 4-vector for the incoming photon

(etc.), and the ‘slash’ notation ✁q ≡ qλγλ. Spin and momentum labels have been dropped, i.e. more

completely, for example, ū4 = ū(s4)(p4) with two possible spin states (s4 = 1, 2). (Implicitly, the

mc factor is multiplied by the identity matrix.)

Figure 1: Feynman diagram of the two lowest-order (i.e. 2-vertex) processes contributing to
Compton scattering (Griffths 2008, p246). Associated with the diagram on the left is an amplitude
M1.

Integration sends q → (p1−p3), and we drop the factor (2π)4 δ4(p1+p2−p3−p4). Then noting

that for fixed index µ the quantity ǫµ(2) is just a scalar (and ditto ǫ∗κ(3)) so that ǫµ(2)ū4 = ū4 ǫµ(2)

(etc.), the amplitude associated with diagram 1 can be written

M1 =
g2e

(p1 − p3)2 −m2c2
[ū4 ✁ǫ2 (✁p1 − ✁p3 +mc) u1 ✁ǫ

∗

3 ] , (2)
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where ✁ǫ2 ≡ ǫµ(2)γ
µ. Analogous steps for the second diagram give amplitude

M2 =
g2e

(p1 + p2)2 −m2c2
[ū4 ✁ǫ

∗

3 (✁p1 + ✁p2 +mc) u1 ✁ǫ2 ] . (3)

To evaluate the cross section for Compton scattering the quantity

|M|2 = M1M
∗

1 +M2M
∗

2 +M1M
∗

2 +M2M
∗

1 (4)

is needed. After some manipulation one obtains

M1M
∗

1 = A2 ū4 ✁ǫ2 [✁p1 − ✁p3 + mc] ✁ǫ
∗

3 u1 ū1 ✁ǫ3 [✁p1 − ✁p3 + mc] ✁ǫ
∗

2 u4 , (5)

M2M
∗

2 = B2 ū4 ✁ǫ
∗

3 [✁p1 + ✁p2 + mc] ✁ǫ2 u1 ū1 ✁ǫ
∗
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∗
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∗

3 u1 ū1 ✁ǫ
∗
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∗

1 = AB ū4 ✁ǫ
∗

3 [✁p1 + ✁p2 + mc] ✁ǫ2 u1 ū1 ✁ǫ3 [✁p1 − ✁p3 + mc] ✁ǫ
∗

2 u4 , (8)

where

A =
g2e

(p1 − p3)2 −m2c2
=

g2e
−2p1 · p3

, (9)

B =
g2e

(p1 + p2)2 −m2c2
=

g2e
2p1 · p2

(10)

(because p21 = m2c2, p22 = p23 = 0).

Then averaging over the initial spin states and summing over final spin states, one obtains the four

contributions

〈|M1|
2〉 =

A2

4
QµλQνκ Tr

[
γµ (✁p1 − ✁p3 +mc) γν (✁p1 +mc) γκ (✁p1 − ✁p3 +mc) γλ (✁p4 +mc)

]
, (11)
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2〉 =

B2

4
QµλQνκ Tr

[
γµ (✁p1 + ✁p2 +mc) γν (✁p1 +mc) γκ (✁p1 + ✁p2 +mc) γλ (✁p4 +mc)

]
, (12)
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∗

2〉 =
AB

4
QµλQνκ Tr

[
γµ (✁p1 − ✁p3 +mc) γν (✁p1 +mc) γλ (✁p1 + ✁p2 +mc) γκ (✁p4 +mc)

]
,

(13)

〈M2M
∗

1〉 =
AB

4
QµλQνκ Tr

[
γµ (✁p1 + ✁p2 +mc) γν (✁p1 +mc) γλ (✁p1 − ✁p3 +mc) γκ (✁p4 +mc)

]
,

(14)

to

〈M2〉 = 〈|M1|
2〉+ 〈|M2|

2〉+ 〈M1M
∗

2〉+ 〈M2M
∗

1〉 . (15)

In Eqs. (11-14) the tensor Qµλ is defined

Qµλ =
∑

s=1,2

ǫ(s)µ ǫ
(s)∗
λ ,
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where the photon polarization vector ǫµ = (ǫ0, ǫ) with ǫ0 = 0. The completeness relation (for the

photon polarization three vectors) is

∑

s=1,2

ǫ
(s)
i ǫ

(s)∗
j = δij − p̂ip̂j (16)

where p̂i is the unit vector p̂i = pi/|pi| (no summation). Hence

Qµλ =

{

0 , if µ = 0 or λ = 0

δµλ − p̂µp̂λ , otherwise .
(17)

Eqns. (11–17) concur with the solution manual written by D. Griffiths (available at www.academia.edu

and elsewhere).

Evaluation of 〈|M|2〉 in terms of Mandelstam variables, using FORM

It can be seen from Eqs. (11, 12) that 〈|M1|
2〉 and 〈|M2|

2〉 are equivalent under the substitution

p2 ↔ −p3 (or s ↔ u in terms of the Mandelstam variables s ≡ (p1 + p2)
2 and u ≡ (p2 − p4)

2 used

below), and the same symmetry links 〈M1M
∗

2〉 and 〈M2M
∗

1〉. Puzzlingly, that symmetry can be

seen at one point in the output of the following FORM program, but, in the ultimate expression,

the expected symmetry is not upheld. The final result for 〈|M|2〉, named “sum” in the FORM

program below, is incorrect.

*** compton_scattering.frm JDW 23 Oct. 2019 ***

Vectors p1, p2, p3, p4;

Symbols m,s,u,[ge^4],[2ge^4];

Symbols [1/(s-m^2)],[1/(s-m^2)^2],[1/(u-m^2)],[1/(u-m^2)^2],[1/(s-m^2)/(u-m^2)];

Indices alpha,beta,gamma,delta,rho,kappa,lambda,mu,nu;

Off Statistics;

Local traceM1M1 = d_(mu,lambda)*d_(nu,kappa)

*g_(1,mu)*(g_(1,p1)-g_(1,p3)+m)

*g_(1,nu)*(g_(1,p1)+m)

*g_(1,kappa)*(g_(1,p1)-g_(1,p3)+m)

*g_(1,lambda)*(g_(1,p4)+m);

Local traceM2M2 = d_(mu,lambda)*d_(nu,kappa)

*g_(2,mu)*(g_(2,p1)+g_(2,p2)+m)

*g_(2,nu)*(g_(2,p1)+m)

*g_(2,kappa)*(g_(2,p1)+g_(2,p2)+m)

https://www.academia.edu/3851437/Griffiths-Complete_Solutions_Manual_Introduction_To_Elementary_Particles.pdf
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*g_(2,lambda)*(g_(2,p4)+m);

Local traceM1M2str = d_(mu,lambda)*d_(nu,kappa)

*g_(3,mu)*(g_(3,p1)-g_(3,p3)+m)

*g_(3,nu)*(g_(3,p1)+m)

*g_(3,lambda)*(g_(3,p1)+g_(3,p2)+m)

*g_(3,kappa)*(g_(3,p4)+m);

Local traceM2M1str = d_(mu,lambda)*d_(nu,kappa)

*g_(4,mu)*(g_(4,p1)+g_(4,p2)+m)

*g_(4,nu)*(g_(4,p1)+m)

*g_(4,lambda)*(g_(4,p1)-g_(4,p3)+m)

*g_(4,kappa)*(g_(4,p4)+m);

Local M1M1 = div_(1,2)*[2ge^4]*traceM1M1*div_(1,4)*(-1/(2*p1.p3))^2;

Local M2M2 = div_(1,2)*[2ge^4]*traceM2M2*div_(1,4)*( 1/(2*p1.p2))^2;

Local M1M2str = div_(1,2)*[2ge^4]*traceM1M2str*div_(1,4)*(-1/(2*p1.p3))*(1/(2*p1.p2));

Local M2M1str = div_(1,2)*[2ge^4]*traceM2M1str*div_(1,4)*(-1/(2*p1.p3))*(1/(2*p1.p2));

Local sum=M1M1+M2M2+M1M2str+M2M1str;

Trace4,1;

Trace4,2;

Trace4,3;

Trace4,4;

.sort;

repeat;

id p2.p2=0;

id p3.p3=0;

id p1.p1=m^2;

id p4.p4=m^2;

endrepeat;

.sort;
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*** Introduce Mandelstam variables.

repeat;

id 1/(p1.p2)=2/(s-m^2);

id 1/(p1.p3)=-2/(u-m^2);

id p1.p4 = (u+s)/2;

id p2.p3=(u+s)/2-m^2;

id p2.p4 = (m^2-u)/2;

id p3.p4 = (s-m^2)/2;

endrepeat;

.sort;

repeat;

id s/(s-m^2)=1+m^2/(s-m^2);

endrepeat;

.sort;

repeat;

id 1/(s - m^2)/(s + m^2)=1/(s^2-m^4);

endrepeat;

.sort;

Bracket [2ge^4],m;

Print;

.sort;

.end;

Here are some selected outputs from the program, that present a puzzle. Prior to the complete

conversion into Mandelstam variables

traceM1M1 =

+ m^2 * ( - 16*u - 80*p1.p3 )

+ m^4 * ( 48 )

+ 16*p1.p3*s;
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traceM2M2 =

+ m^2 * ( - 16*s + 80*p1.p2 )

+ m^4 * ( 48 )

- 16*p1.p2*u;

showing the expected symmetry of |M1|
2 and |M2|

2. However upon completion

M1M1 =

+ [2ge^4] * ( - 1/(u - m^2)*s )

+ m^2*[2ge^4] * ( 5/(u - m^2) - 2/(u - m^2)/(u - m^2)*u )

+ m^4*[2ge^4] * ( 6/(u - m^2)/(u - m^2) );

M2M2 =

+ [2ge^4] * ( - 1/(s - m^2)*u )

+ m^2*[2ge^4] * ( 3/(s - m^2) )

+ m^4*[2ge^4] * ( 4/(s - m^2)/(s - m^2) );

such that the expected symmetry is not evident. The balance of the output

M1M2str =

+ [2ge^4] * ( - 1 + 1/(u - m^2)*u - 1/(s - m^2)*u + 1/(s - m^2)/(u -

m^2)*u^2 )

+ m^2*[2ge^4] * ( 1/(s - m^2) - 1/(s - m^2)/(u - m^2)*u )

+ m^4*[2ge^4] * ( 4/(s - m^2)/(u - m^2) );

M2M1str =

+ [2ge^4] * ( - 1 + 1/(u - m^2)*u - 1/(s - m^2)*u + 1/(s - m^2)/(u -

m^2)*u^2 )

+ m^2*[2ge^4] * ( 1/(s - m^2) - 1/(s - m^2)/(u - m^2)*u )

+ m^4*[2ge^4] * ( 4/(s - m^2)/(u - m^2) );



7

sum =

+ [2ge^4] * ( - 2 + 2/(u - m^2)*u - 1/(u - m^2)*s - 3/(s - m^2)*u + 2

/(s - m^2)/(u - m^2)*u^2 )

+ m^2*[2ge^4] * ( 5/(u - m^2) - 2/(u - m^2)/(u - m^2)*u + 5/(s - m^2)

- 2/(s - m^2)/(u - m^2)*u )

+ m^4*[2ge^4] * ( 6/(u - m^2)/(u - m^2) + 8/(s - m^2)/(u - m^2) + 4/(s

- m^2)/(s - m^2) );

does show the expected symmetry of 〈M1M
∗

2〉, 〈M2M
∗

1〉, but, judged against Millar’s (2014)

result

the present result (from FORM) for 〈|M|2〉 (i.e. “sum”), while promising, is not quite correct.
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